Clap/eDSLState/ConstraintSystem.lean
@@ -1,0 +1,141 @@
+import Clap.eDSLState.Circuit
+import Clap.eDSLState.Varstore
+-- import Clap.eDSLState.Convert.Specialised
+
+namespace Clap
+
+open HashConsM
+
+structure ConstraintSystem (p : ℕ) where
+  eq0s : Array ExprRef
+  σ : HashConsSt p
+
+namespace ConstraintSystem
+
+variable {p : ℕ} (cs: ConstraintSystem p)
+
+def runSpec (trace : Array (ZMod p)) : Bool :=
+  cs.eq0s.all (λ expr => [.ofArray (trace.zipIdx.map Prod.swap), cs.σ|expr] == .some 0)
+
+-- TODO prove equivalent to runSpec
+-- TODO make evalWithArrayCache to avoid the conversion and prove equivalent to evalWithCache
+def run (trace : Array (ZMod p)) : Bool :=
+  let max := cs.eq0s.max?
+  match max with
+  | .none => true
+  | .some max =>
+    let cache := Expr.evalWithCache (.ofArray (trace.zipIdx.map Prod.swap)) #[] ⦃max, cs.σ⦄
+    cs.eq0s.all (λ expr => cache[expr]? == .some (0 : ZMod p))
+
+def num_constraints : Gate → ℕ
+  | .eq0 _ => 1
+  | .share _ => 1
+  | .isZero _ => 2
+  | .num2bits w _ => w + 1
+  | .fpmul w k a b p' => 42
+
+end ConstraintSystem
+
+def HashConsM.mkBits2num {p : ℕ} (bits : Array ExprRef) : HashConsM p ExprRef := do
+  let init ← mkConstant 0
+  bits.foldrM (λ bit acc => do mkAdd bit (←mkMul (←mkConstant 2) acc)) init
+
+-- def rangeCheckCircuit (w : ℕ) {k : ℕ} (vec : Vector ExprRef k) : HashConsM p _ :=
+
+-- def fpMul_circuit
+--   {p k w : ℕ}
+--   (a b p' : Vector ExprRef k) : HashConsM p (Array ExprRef × ℕ) := do
+--   _
+
+def eq0ToCs {p} (constraints : Array ExprRef) (numAlloc : ℕ) (expr : ExprRef) :
+  HashConsM p (Array ExprRef × ℕ) :=
+  return (constraints.push expr, numAlloc)
+
+def shareToCs {p}
+  (constraints : Array ExprRef) (numAlloc : ℕ) (expr : ExprRef)
+:
+  HashConsM p (ExprRef × Array ExprRef × ℕ)
+:= do
+  let v ← mkVar numAlloc
+  let s ← expr - v
+  return (v, constraints.push s, numAlloc + 1)
+
+def isZeroToCs {p} (constraints : Array ExprRef) (numAlloc : ℕ) (expr : ExprRef) :
+  HashConsM p (ExprRef × Array ExprRef × ℕ) := do
+  let inv ← mkVar numAlloc
+  let o ← mkVar (numAlloc + 1)
+  let constraint1 ← (←((←mkConstant 1) - (←inv * expr))) - o
+  let constraint2 ← o * expr
+  return (o, constraints.append #[constraint1, constraint2], numAlloc + 2)
+
+def num2bitsToCs {p} (cs : Array ExprRef) (numAlloc width : ℕ) (expr : BoundRef p) :
+  HashConsM p (Array ExprRef × Array ExprRef × ℕ) := do
+  let bits ← (Array.range width).mapM (λ idx => mkVar (numAlloc + idx))
+  let bit_constraints ← bits.mapM (λ bit => do bit * (←(←mkConstant 1) - bit)) -- equivalent to assert_bit_e
+  let value_constraint ← (←mkBits2num bits) - expr
+  let constraints := bit_constraints.push value_constraint
+  return (bits, cs.append constraints, numAlloc + width)
+
+def offsetSince (threshold idx offset : ℕ) : ℕ :=
+  if idx < threshold then idx else idx + offset
+
+/--
+Not to be confused with Colonel Allocs.
+-/
+def privateAllocs (gate : Gate) : ℕ :=
+  match gate with
+  | .eq0 e => 0
+  | .share e => 0
+  | .isZero e => 1
+  | .num2bits w e => 0
+  | .fpmul w k a b p' => 42
+
+def offsetIdx (circuit : Circuit) : ℕ → ℕ :=
+  (·.1) <| circuit.foldr (init := (id, circuit.numAllocStep))
+    fun gate (f, threshold) ↦
+      let privateAllocs := privateAllocs gate
+      let publicAllocs := gate.numAllocStep
+      /-
+        [public₁, public₂]
+                         ^ threshold
+        ^ threshold - publicAllocs
+        [priv₁, priv₂, public₁, public₂]
+      -/
+      let nextThreshold := threshold - publicAllocs
+      -- dbg_trace s!"t: {threshold}\npriv: {privateAllocs}\npublic: {publicAllocs}\nnextT: {nextThreshold}"
+      let yourFace := fun idx ↦ offsetSince nextThreshold (f idx) privateAllocs
+      -- dbg_trace s!"{List.range 50 |>.map yourFace}"
+      (yourFace, nextThreshold)
+
+-- def hashConsStateButBetter (σ : HashConsSt p)
+
+def ranDom (n : ℕ) : Gate :=
+  match n with
+  | 1 => .isZero 0
+  | 2 => .eq0 0
+  | 3 => .share 0
+  | _ => .num2bits 5 5
+
+def yourFace : Circuit := #[4, 1, 2, 1, 2, 1, 3, 2, 2, 3, 2, 3, 1, 4, 1, 4, 2, 2, 3, 2].map ranDom
+-- [0, 1, 2, 3, 4, 6, 8, 10, 11, 12, 13, 14, 16, 17, 18, 19, 20, 21, 23, 24, 25, 26, 27, 28]
+#eval yourFace.numAllocStep
+#eval (List.range yourFace.numAllocStep |>.map (offsetIdx yourFace))
+-- #eval List.range yourFace.size |>.map (offsetIdx yourFace)
+
+open HashConsM in
+def Circuit.toCs {p : ℕ} (circuit : Circuit) (σ : HashConsSt p) (numInputs : ℕ)
+:
+  ConstraintSystem p
+:=
+  let ((eq0s, _numAlloc), σPost) :=
+    (circuit.foldlM (m := HashConsM p) (λ (eq0s, numAlloc) gate => do
+      match gate with
+      | .eq0 expr => eq0ToCs eq0s numAlloc expr
+      | .share expr => return (←shareToCs eq0s numAlloc expr).2
+      | .isZero expr => return (←isZeroToCs eq0s numAlloc expr).2
+      | .num2bits width expr => return (←num2bitsToCs eq0s numAlloc width expr).2
+      | .fpmul w k a b p' => sorry
+    ) (Array.emptyWithCapacity (circuit.map ConstraintSystem.num_constraints).sum , numInputs)).run σ
+  ⟨eq0s, σPost⟩
+
+end Clap
