Clap/eDSLState/WitnessGenerator/fpMul.lean
@@ -7,17 +7,18 @@ section Andrew
 
 open CompPoly
 
-variable {p : ℕ}
+variable {p : ℕ} {var : Type} [inst : Fact (Nat.Prime p)] [inst' : Fact (p > 2)]
 
 namespace WitnessGenerator
 
 def toCompPoly {k : ℕ} (vec : Vector (ZMod p) k) : CPolynomial (ZMod p) :=
   List.foldr (fun i p ↦ p + CPolynomial.C (vec[i]) * CPolynomial.X ^ i.1) 0 (List.finRange k)
 
-def fpMul {p : ℕ}
-  (cache : ValueCache p) (trace : Array (ZMod p)) (width : ℕ) (expr : ExprRef) : Array (ZMod p) :=
-  let ab := toCompPoly (a.map (Exp.eval)) * toCompPoly (b.map (Exp.eval))
-  _
+def fpMul
+  (cache : ValueCache p) (trace : Array (ZMod p))
+  (w k : ℕ) (a b p' : Vector ExprRef k) : Array (ZMod p) :=
+  let ab := toCompPoly (a.map (cache[·]!.get!)) * toCompPoly (b.map (cache[·]!.get!))
+  sorry
 
 end WitnessGenerator
 
